lean/src/bpf/absint/regs.lean
@@ -3,6 +3,7 @@ Copyright (c) 2021 The UNSAT Group. All rights reserved.
 Released under Apache 2.0 license as described in the file LICENSE.
 Authors: Luke Nelson, Xi Wang
 -/
+import .value
 import bpf.basic
 import data.domain.basic
 import data.domain.bv
@@ -17,34 +18,48 @@ namespace absint
 An abstraction of BPF registers.
 -/
 class regs_abstr (α : Type*) extends
-  has_γ (bpf.reg → bpf.i64) α,
-  abstr_top (bpf.reg → bpf.i64) α,
-  abstr_le (bpf.reg → bpf.i64) α,
-  abstr_join (bpf.reg → bpf.i64) α α :=
+  has_γ (bpf.reg → bpf.value) α,
+  abstr_top (bpf.reg → bpf.value) α,
+  abstr_le (bpf.reg → bpf.value) α,
+  abstr_join (bpf.reg → bpf.value) α α :=
 
 -- Do a reg-reg ALU op.
 (do_alu (op : bpf.ALU) (dst src : bpf.reg) :
-  abstr_unary_transfer (bpf.reg → bpf.i64) α
+  abstr_unary_transfer (bpf.reg → bpf.value) α
     (λ cregs, function.update cregs dst (bpf.ALU.doALU op (cregs dst) (cregs src))))
+
+-- Check if an ALU op is legal.
+(do_alu_check (op : bpf.ALU) (dst src : bpf.reg) :
+  abstr_unary_test (bpf.reg → bpf.value) α
+    (λ cregs, bpf.ALU.doALU_check op (cregs dst) (cregs src) = tt))
 
 -- Do an ALU op with an immediate.
 (do_alu_imm (op : bpf.ALU) (dst : bpf.reg) (imm : lsbvector 64) :
-  abstr_unary_transfer (bpf.reg → bpf.i64) α
-    (λ cregs, function.update cregs dst (bpf.ALU.doALU op (cregs dst) imm.nth)))
+  abstr_unary_transfer (bpf.reg → bpf.value) α
+    (λ cregs, function.update cregs dst (bpf.ALU.doALU op (cregs dst) (bpf.value.scalar imm.nth))))
+
+-- Check if an ALU op is legal.
+(do_alu_imm_check (op : bpf.ALU) (dst : bpf.reg) (imm : lsbvector 64) :
+  abstr_unary_test (bpf.reg → bpf.value) α
+    (λ cregs, bpf.ALU.doALU_check op (cregs dst) (bpf.value.scalar imm.nth) = tt))
+
+-- Check if a JMP is legal on some operands.
+(do_jmp_check (op : bpf.JMP) (dst src : bpf.reg) :
+  abstr_unary_test (bpf.reg → bpf.value) α
+    (λ cregs, bpf.JMP.doJMP_check op (cregs dst) (cregs src) = tt))
 
 -- Invert a reg/reg JMP op whose condition is true
 (invert_jmp_tt (op : bpf.JMP) (dst src : bpf.reg) :
-  abstr_unary_inversion (bpf.reg → bpf.i64) α (with_bot α)
-    (λ (cregs : bpf.reg → bpf.i64), bpf.JMP.doJMP op (cregs dst) (cregs src) = tt))
+  abstr_unary_inversion (bpf.reg → bpf.value) α (with_bot α)
+    (λ (cregs : bpf.reg → bpf.value), bpf.JMP.doJMP op (cregs dst) (cregs src) = tt))
 
--- Test if a register `reg` cannot be equal to `val`.
-(test_reg_neq (reg : bpf.reg) (val : bpf.i64) :
-  abstr_unary_test (bpf.reg → bpf.i64) α
-    (λ cregs, cregs reg ≠ val))
+(is_scalar (r : bpf.reg) :
+  abstr_unary_test (bpf.reg → bpf.value) α
+    (λ (cregs : bpf.reg → bpf.value), (cregs r).is_scalar))
 
 namespace nonrelational
 
-variables {β : Type} [bv_abstr 64 β]
+variables {β : Type} [value_abstr β]
 open has_γ abstr_top abstr_le abstr_join
 
 abbreviation aregs (β : Type) := vector β bpf.nregs
@@ -52,10 +67,10 @@ abbreviation aregs (β : Type) := vector β bpf.nregs
 def interpret (abs : aregs β) : bpf.reg → β :=
 λ k, (abs.nth k.to_fin)
 
-instance : has_γ (bpf.reg → bpf.i64) (aregs β) :=
-{ γ := λ (l : aregs β) (f : bpf.reg → bpf.i64),
+instance : has_γ (bpf.reg → bpf.value) (aregs β) :=
+{ γ := λ (l : aregs β) (f : bpf.reg → bpf.value),
     ∀ k, γ (interpret l k) (f k),
-  abstract := λ (f : bpf.reg → bpf.i64),
+  abstract := λ (f : bpf.reg → bpf.value),
     (fin_enum.to_vector bpf.reg).map (abstract ∘ f),
   abstract_correct := by {
     intros f r,
@@ -65,20 +80,20 @@ instance : has_γ (bpf.reg → bpf.i64) (aregs β) :=
 instance : has_le (aregs β) :=
 ⟨ λ a b, ∀ k, interpret a k ≤ interpret b k ⟩
 
-instance : abstr_le (bpf.reg → bpf.i64) (aregs β) :=
+instance : abstr_le (bpf.reg → bpf.value) (aregs β) :=
 { dec_le     := infer_instance,
   le_correct := by {
     intros x y h₁ f h₂ r,
     apply le_correct (h₁ r) (h₂ r) } }
 
-instance : abstr_top (bpf.reg → bpf.i64) (aregs β) :=
+instance : abstr_top (bpf.reg → bpf.value) (aregs β) :=
 { top := vector.repeat ⊤ _,
   top_correct := by {
     intros _ _,
     simp only [interpret, vector.nth_repeat],
     apply top_correct } }
 
-instance : abstr_join (bpf.reg → bpf.i64) (aregs β) (aregs β) :=
+instance : abstr_join (bpf.reg → bpf.value) (aregs β) (aregs β) :=
 { join := λ x y, vector.map₂ join x y,
   join_correct := by {
     rintros x y f h₁ r,
@@ -91,49 +106,20 @@ instance : abstr_join (bpf.reg → bpf.i64) (aregs β) (aregs β) :=
       exact h₁ r } } }
 
 /-- Test whether `reg` can be `val`. -/
-def test_reg (abs : aregs β) (reg : bpf.reg) (val : bpf.i64) : bool :=
+def test_reg (abs : aregs β) (reg : bpf.reg) (val : bpf.value) : bool :=
 γ (interpret abs reg) val
 
-def test_reg_neq (reg : bpf.reg) (val : bpf.i64) :
-  abstr_unary_test (bpf.reg → bpf.i64) (aregs β) (λ cregs, cregs reg ≠ val) :=
-{ test       := λ (l : aregs β), !to_bool (γ (interpret l reg) val),
-  test_sound := by {
-    intros _ _ test_tt gamma,
-    simp only [bnot_eq_true_eq_eq_ff, bool.to_bool_not, to_bool_ff_iff] at test_tt ⊢,
-    contrapose! test_tt,
-    subst test_tt,
-    apply gamma } }
-
-/-- Abstract transfer function for ALU operations. -/
-private def transfer_ALU : Π (op : bpf.ALU), abstr_binary_transfer bpf.i64 β β (bpf.ALU.doALU64 op)
-| bpf.ALU.ADD  := bv_abstr.add
-| bpf.ALU.AND  := bv_abstr.and
-| bpf.ALU.ARSH := bv_abstr.ashr
-| bpf.ALU.DIV  := bv_abstr.udiv
-| bpf.ALU.LSH  := bv_abstr.shl
-| bpf.ALU.MOD  := bv_abstr.urem
-| bpf.ALU.MOV  := { op := λ _ y, y, correct := by { intros, assumption } }
-| bpf.ALU.MUL  := bv_abstr.mul
-| bpf.ALU.OR   := bv_abstr.or
-| bpf.ALU.RSH  := bv_abstr.lshr
-| bpf.ALU.XOR  := bv_abstr.xor
-| _ :=
-  { op      := λ _ _, ⊤,
-    correct := by {
-      intros,
-      apply top_correct } }
-
 private def do_alu (op : bpf.ALU) (dst src : bpf.reg) :
-  abstr_unary_transfer (bpf.reg → bpf.i64) (aregs β)
+  abstr_unary_transfer (bpf.reg → bpf.value) (aregs β)
     (λ cregs, function.update cregs dst (bpf.ALU.doALU op (cregs dst) (cregs src))) :=
-{ op      := λ (l : aregs β), l.update_nth dst.to_fin ((transfer_ALU op).op (interpret l dst) (interpret l src)),
+{ op      := λ (l : aregs β), l.update_nth dst.to_fin ((value_abstr.doALU op).op (interpret l dst) (interpret l src)),
   correct := by {
     intros _ _ h₁ r,
     simp only [function.update],
     split_ifs with h,
     { subst h,
       simp only [interpret, option.get_or_else_some, vector.nth_update_nth_same],
-      exact (transfer_ALU op).correct (h₁ r) (h₁ src) },
+      exact (value_abstr.doALU op).correct (h₁ r) (h₁ src) },
     { simp only [interpret],
       rw [vector.nth_update_nth_of_ne _],
       exact h₁ r,
@@ -142,16 +128,16 @@ private def do_alu (op : bpf.ALU) (dst src : bpf.reg) :
       apply bpf.reg.to_fin_inj h } } }
 
 def do_alu_imm (op : bpf.ALU) (dst : bpf.reg) (imm : lsbvector 64) :
-  abstr_unary_transfer (bpf.reg → bpf.i64) (aregs β)
-    (λ cregs, function.update cregs dst (bpf.ALU.doALU op (cregs dst) imm.nth)) :=
-{ op      := λ (l : aregs β), l.update_nth dst.to_fin ((transfer_ALU op).op (interpret l dst) (abstract imm.nth)),
+  abstr_unary_transfer (bpf.reg → bpf.value) (aregs β)
+    (λ cregs, function.update cregs dst (bpf.ALU.doALU op (cregs dst) (bpf.value.scalar imm.nth))) :=
+{ op      := λ (l : aregs β), l.update_nth dst.to_fin ((value_abstr.doALU op).op (interpret l dst) (abstract (bpf.value.scalar imm.nth))),
   correct := by {
     intros _ _ h₁ r,
     simp only [function.update],
     split_ifs with h,
     { subst h,
       simp only [interpret, option.get_or_else_some, vector.nth_update_nth_same],
-      exact (transfer_ALU op).correct (h₁ r) (abstract_correct _) },
+      exact (value_abstr.doALU op).correct (h₁ r) (abstract_correct _) },
     { simp only [interpret],
       rw [vector.nth_update_nth_of_ne _],
       exact h₁ r,
@@ -159,41 +145,21 @@ def do_alu_imm (op : bpf.ALU) (dst : bpf.reg) (imm : lsbvector 64) :
       symmetry,
       apply bpf.reg.to_fin_inj h } } }
 
-/-- Abstract transfer function for ALU operations. -/
-def transfer_JMP : ∀ (op : bpf.JMP), abstr_binary_inversion bpf.i64 β (with_bot β) (λ x y, bpf.JMP.doJMP op x y = tt)
-| bpf.JMP.JEQ := by {
-  convert abstr_meet.invert_equality,
-  simp only [bpf.JMP.doJMP, to_bool_iff],
-  apply_instance }
-| bpf.JMP.JLT := by {
-  convert bv_abstr.lt,
-  simp only [bpf.JMP.doJMP, to_bool_iff] }
-| bpf.JMP.JGT := by {
-  convert bv_abstr.gt,
-  simp only [bpf.JMP.doJMP, to_bool_iff] }
-| bpf.JMP.JLE := by {
-  convert bv_abstr.le,
-  simp only [bpf.JMP.doJMP, to_bool_iff] }
-| bpf.JMP.JGE := by {
-  convert bv_abstr.ge,
-  simp only [bpf.JMP.doJMP, to_bool_iff] }
-| _ := abstr_binary_inversion.trivial
-
 def invert_jmp_tt (op : bpf.JMP) (dst src : bpf.reg) :
-  abstr_unary_inversion (bpf.reg → bpf.i64) (aregs β) (with_bot (aregs β))
-    (λ (cregs : bpf.reg → bpf.i64), bpf.JMP.doJMP op (cregs dst) (cregs src) = tt) :=
+  abstr_unary_inversion (bpf.reg → bpf.value) (aregs β) (with_bot (aregs β))
+    (λ (cregs : bpf.reg → bpf.value), bpf.JMP.doJMP op (cregs dst) (cregs src) = tt) :=
 { inv := λ (l : aregs β),
-    (let z := (transfer_JMP op).inv (interpret l dst) (interpret l src) in do
+    (let z := (value_abstr.doJMP_tt op).inv (interpret l dst) (interpret l src) in do
       dst' ← z.1,
       src' ← z.2,
       pure $ (l.update_nth dst.to_fin dst').update_nth src.to_fin src'),
   correct := by {
     intros regs regs' h₁ jmp_eq,
     simp only,
-    have h₃ := (transfer_JMP op).correct (h₁ dst) (h₁ src) jmp_eq,
-    cases ((transfer_JMP op).inv (interpret regs' dst) (interpret regs' src)).1 with dst',
+    have h₃ := (value_abstr.doJMP_tt op).correct (h₁ dst) (h₁ src) jmp_eq,
+    cases ((value_abstr.doJMP_tt op).inv (interpret regs' dst) (interpret regs' src)).1 with dst',
     { rcases h₃ with ⟨⟨⟩, -⟩ },
-    cases ((transfer_JMP op).inv (interpret regs' dst) (interpret regs' src)).2 with src',
+    cases ((value_abstr.doJMP_tt op).inv (interpret regs' dst) (interpret regs' src)).2 with src',
     { rcases h₃ with ⟨-, ⟨⟩⟩ },
     simp only [option.some_bind],
     intros r,
@@ -215,10 +181,13 @@ def invert_jmp_tt (op : bpf.JMP) (dst src : bpf.reg) :
     exact h₁ r } }
 
 instance : regs_abstr (aregs β) :=
-{ do_alu         := do_alu,
-  do_alu_imm     := do_alu_imm,
-  invert_jmp_tt  := invert_jmp_tt,
-  test_reg_neq   := test_reg_neq }
+{ do_alu           := do_alu,
+  do_alu_check     := sorry,
+  do_alu_imm       := do_alu_imm,
+  do_alu_imm_check := sorry,
+  invert_jmp_tt    := invert_jmp_tt,
+  is_scalar        := sorry,
+  do_jmp_check     := sorry }
 
 end nonrelational
 end absint
