lean/src/bpf/absint/value.lean
@@ -1,0 +1,45 @@
+/-
+Copyright (c) 2021 The UNSAT Group. All rights reserved.
+Released under Apache 2.0 license as described in the file LICENSE.
+Authors: Luke Nelson, Xi Wang
+-/
+import data.domain.basic
+import data.domain.bv
+import bpf.basic
+
+namespace absint
+
+/--
+Class for abstractions of values of BPF registers.
+-/
+class value_abstr (α : Type*) extends
+  has_decidable_γ bpf.value α,
+  abstr_le bpf.value α,
+  abstr_top bpf.value α,
+  abstr_join bpf.value α α,
+  abstr_meet bpf.value α (with_bot α) :=
+
+(doALU (op : bpf.ALU) :
+  abstr_binary_transfer bpf.value α α (bpf.ALU.doALU op))
+
+(doJMP_tt (op : bpf.JMP) :
+  abstr_binary_inversion bpf.value α (with_bot α) (λ x y, op.doJMP x y = tt))
+
+inductive avalue (β : Type) : Type
+| scalar : β → avalue
+| pointer : bpf.memregion → β → avalue
+
+namespace avalue
+
+variables {β : Type} [bv_abstr 64 β]
+
+instance : has_γ bpf.value (avalue β) :=
+sorry
+
+instance : abstr_le bpf.value (avalue β) := sorry
+
+instance : value_abstr (avalue β) :=
+sorry
+
+end avalue
+end absint
