lean/src/bpf/se/symbolic_value.lean
@@ -1,0 +1,103 @@
+/-
+Copyright (c) 2021 The UNSAT Group. All rights reserved.
+Released under Apache 2.0 license as described in the file LICENSE.
+Authors: Luke Nelson, Xi Wang
+-/
+import bpf.basic
+import smt.factory
+
+namespace bpf
+namespace cfg
+namespace se
+universe u
+
+variables {β γ : Type u} [smt.factory β γ] [smt.add_factory β γ] [smt.const_factory β γ]
+  [smt.eq_factory β γ] [smt.not_factory β γ] [smt.and_factory β γ] [smt.redor_factory β γ] [smt.ult_factory β γ]
+  [smt.ule_factory β γ] [smt.slt_factory β γ] [smt.sle_factory β γ]
+open smt.add_factory smt.const_factory smt.eq_factory smt.not_factory smt.and_factory smt.redor_factory smt.ult_factory
+     smt.slt_factory smt.sle_factory smt.ule_factory
+
+/-- Symbolic values of BPF registers -/
+inductive symvalue (β : Type u)
+| pointer : bpf.memregion → β → symvalue
+| scalar : β → symvalue
+| unknown : erased value → symvalue
+
+namespace symvalue
+
+inductive sat (g : γ) : (symvalue β) → bpf.value → Prop
+| sat_pointer {r : bpf.memregion} {off : β} {off_v : bpf.i64} :
+  factory.sat g off (⟨64, off_v⟩ : Σ (n : ℕ), fin n → bool) →
+  sat (symvalue.pointer r off) (value.pointer r off_v)
+| sat_scalar {val : β} {val_v : bpf.i64} :
+  factory.sat g val (⟨64, val_v⟩ : Σ (n : ℕ), fin n → bool) →
+  sat (symvalue.scalar val) (value.scalar val_v)
+
+instance : factory bpf.value (symvalue β) γ :=
+{ sat          := sat,
+  sat_of_le    := sorry,
+  init_f       := factory.init_f (Σ (n : ℕ), fin n → bool) β,
+  default      := ⟨symvalue.unknown $ erased.mk $ value.scalar 0⟩,
+  denote       := sorry,
+  denote_sound := sorry }
+
+def mk_scalar (imm : lsbvector 64) : state γ (symvalue β) :=
+symvalue.scalar <$> mk_const imm
+
+theorem sat_mk_scalar ⦃g g' : γ⦄ ⦃e₁ : symvalue β⦄ ⦃imm : lsbvector 64⦄ :
+  (mk_scalar imm).run g = (e₁, g') →
+  sat g e₁ (bpf.value.scalar imm.nth) :=
+sorry
+
+def mk_unknown (v : erased value) : state γ (symvalue β) :=
+pure (symvalue.unknown v)
+
+theorem sat_mk_unknown ⦃g g' : γ⦄ ⦃e₁ : symvalue β⦄ ⦃v : erased bpf.value⦄ :
+  (mk_unknown v).run g = (e₁, g') →
+  sat g e₁ v.out :=
+sorry
+
+def doALU : Π (op : bpf.ALU) (a b : symvalue β), state γ (symvalue β)
+| bpf.ALU.ADD (symvalue.scalar x) (symvalue.scalar y) :=
+  symvalue.scalar <$> mk_add x y
+| _ _ _ := pure (symvalue.unknown $ erased.mk $ value.scalar 0)
+
+theorem sat_doALU ⦃g g' : γ⦄ ⦃op : bpf.ALU⦄ ⦃e₁ e₂ e₃ : symvalue β⦄ ⦃v₁ v₂ : bpf.value⦄ :
+  (doALU op e₁ e₂).run g = (e₃, g') →
+  sat g e₁ v₁ →
+  sat g e₂ v₂ →
+  sat g e₃ (bpf.ALU.doALU op v₁ v₂) :=
+sorry
+
+def doALU_check : Π (op : bpf.ALU) (a b : symvalue β), state γ β
+| _ _ _ := mk_false
+
+theorem sat_doALU_check ⦃g g' : γ⦄ ⦃op : bpf.ALU⦄ ⦃e₁ e₂ : symvalue β⦄ ⦃e₃ : β⦄ ⦃v₁ v₂ : bpf.value⦄ :
+  (doALU_check op e₁ e₂).run g = (e₃, g') →
+  sat g e₁ v₁ →
+  sat g e₂ v₂ →
+  factory.sat g e₃ (⟨1, λ _, bpf.ALU.doALU_check op v₁ v₂ = tt⟩ : Σ (n : ℕ), fin n → bool) :=
+sorry
+
+def doJMP : Π (op : bpf.JMP) (a b : symvalue β), state γ β
+| JMP.JEQ  (symvalue.scalar x) (symvalue.scalar y) := mk_eq x y
+| JMP.JNE  (symvalue.scalar x) (symvalue.scalar y) := mk_eq x y >>= mk_not
+| JMP.JSET (symvalue.scalar x) (symvalue.scalar y) := mk_and x y >>= mk_redor
+| JMP.JLT  (symvalue.scalar x) (symvalue.scalar y) := mk_ult x y
+| JMP.JGT  (symvalue.scalar x) (symvalue.scalar y) := mk_ult y x
+| JMP.JLE  (symvalue.scalar x) (symvalue.scalar y) := mk_ule x y
+| JMP.JGE  (symvalue.scalar x) (symvalue.scalar y) := mk_ule y x
+| JMP.JSLT (symvalue.scalar x) (symvalue.scalar y) := mk_slt x y
+| JMP.JSGT (symvalue.scalar x) (symvalue.scalar y) := mk_slt y x
+| JMP.JSLE (symvalue.scalar x) (symvalue.scalar y) := mk_sle x y
+| JMP.JSGE (symvalue.scalar x) (symvalue.scalar y) := mk_sle y x
+| _ _ _ := mk_true
+
+def doJMP_check : Π (op : bpf.JMP) (a b : symvalue β), state γ β
+| _ (symvalue.scalar x) (symvalue.scalar y) := mk_true
+| _ _ _ := mk_false
+
+end symvalue
+end se
+end cfg
+end bpf
